Remove `sig` and reflect up to `BoundIn.Term`

theories/BoundIn.v
@@ -11,12 +11,12 @@ From LinearCore Require Import
 
 
 Definition Reflect {T} (P : T -> Name.name -> Prop) (p : T -> Map.set) : Prop :=
-  forall t x, P t x <-> Map.In x (p t).
+  forall t, Map.Reflect (P t) (p t).
 Arguments Reflect {T} P p/.
 
 
 
-Definition Strict strict : Name.name -> Prop := Pattern.BoundIn (proj1_sig strict).
+Inductive Strict : Pattern.strict -> Name.name -> Prop :=
   | SArg curried name
       : Strict (Pattern.App curried name) name
   | SRec curried name (bound_earlier : Strict curried name) argument
@@ -26,14 +26,14 @@ Definition Strict strict : Name.name -> Prop := Pattern.BoundIn (proj1_sig stric
 Fixpoint strict s : Map.set :=
   match s with
   | Pattern.Ctr _ => Map.empty
-  | Pattern.App curried argument => Map.add argument tt (strict curried)
+  | Pattern.App curried argument => Map.overriding_add argument tt (strict curried)
   end.
 
 Lemma strict_spec : Reflect Strict strict. Proof.
   split.
-  - intro S. induction S; cbn; apply Map.in_add; [left | right]. { reflexivity. } exact IHS.
-  - intro I. generalize dependent x. induction t; intros; cbn in *. { destruct I as [y M]. invert M. }
-    apply Map.in_add in I as [-> | I]; [left | right]. apply IHt. exact I.
+  - intro I. generalize dependent x. induction t; intros; cbn in *. { destruct I as [y F]. invert F. }
+    apply Map.in_overriding_add in I as [-> | I]; [left | right]. apply IHt. exact I.
+  - intro S. induction S; cbn; apply Map.in_overriding_add; [left | right]. { reflexivity. } exact IHS.
 Qed.
 
 
@@ -53,18 +53,18 @@ Definition pattern p : Map.set :=
 
 Lemma pattern_spec : Reflect Pattern pattern. Proof.
   split.
-  - intro S. invert S; cbn.
-    + apply Map.in_singleton. reflexivity.
-    + apply strict_spec. exact bound_in_strict.
   - intro I. generalize dependent x. induction t; intros; cbn in *.
     + apply Map.in_singleton in I as ->. constructor.
     + constructor. apply strict_spec. exact I.
+  - intro S. invert S; cbn.
+    + apply Map.in_singleton. reflexivity.
+    + apply strict_spec. exact bound_in_strict.
 Qed.
 
 
 
 (* Bound *anywhere* in a term: not only at the top-level (e.g. in a match) but also arbitrarily far from control flow. *)
-Inductive Term : forall (term : Term.term) (name : Name.name), Prop :=
+Inductive Term : Term.term -> Name.name -> Prop :=
   | TMov name
       : Term (Term.Mov name) name
   | TRef name
@@ -86,13 +86,41 @@ Inductive Term : forall (term : Term.term) (name : Name.name), Prop :=
   | TCaO other_cases name (bound_in_other_cases : Term other_cases name) pattern body_if_match
       : Term (Term.Cas pattern body_if_match other_cases) name
   .
+Arguments Term term name.
 
 Fixpoint term t : Map.set :=
   match t with
   | Term.Mov name
   | Term.Ref name => Map.singleton name tt
   | Term.App function arg => Map.set_union (term function) (term arg)
-  | Term.For variable type body => Map.add variable tt (Map.set_union (term type) (term body))
+  | Term.For variable type body => Map.overriding_add variable tt (Map.set_union (term type) (term body))
   | Term.Cas p body_if_match other_cases => Map.set_union (pattern p) (Map.set_union (term body_if_match) (term other_cases))
   | _ => Map.empty
   end.
+
+Lemma term_spec : Reflect Term term. Proof.
+  split.
+  - intro I. generalize dependent x. induction t; intros; simpl term in *.
+    + apply Map.empty_empty in I as [].
+    + apply Map.empty_empty in I as [].
+    + apply Map.empty_empty in I as [].
+    + apply Map.empty_empty in I as [].
+    + apply Map.in_singleton in I as ->. constructor.
+    + apply Map.in_singleton in I as ->. constructor.
+    + apply Map.in_overriding_union in I as [I | I]; [apply TApF | apply TApA]; [apply IHt1 | apply IHt2]; exact I.
+    + apply Map.in_overriding_add in I as [-> | I]. { apply TFoV. }
+      apply Map.in_overriding_union in I as [I | I]; [apply TFoT | apply TFoB]; [apply IHt1 | apply IHt2]; exact I.
+    + apply Map.in_overriding_union in I as [I | I]. { apply TCaP. apply pattern_spec. exact I. }
+      apply Map.in_overriding_union in I as [I | I]; [apply TCaB | apply TCaO]; [apply IHt1 | apply IHt2]; exact I.
+  - intro T. induction T; simpl term in *.
+    + apply Map.in_singleton. reflexivity.
+    + apply Map.in_singleton. reflexivity.
+    + apply Map.in_overriding_union. left. exact IHT.
+    + apply Map.in_overriding_union. right. exact IHT.
+    + apply Map.in_overriding_add. left. reflexivity.
+    + apply Map.in_overriding_add. right. apply Map.in_overriding_union. left. exact IHT.
+    + apply Map.in_overriding_add. right. apply Map.in_overriding_union. right. exact IHT.
+    + apply Map.in_overriding_union. left. apply pattern_spec. exact bound_in_pattern.
+    + apply Map.in_overriding_union. right. apply Map.in_overriding_union. left. exact IHT.
+    + apply Map.in_overriding_union. right. apply Map.in_overriding_union. right. exact IHT.
+Qed.
