theories/Map.v
@@ -8,7 +8,7 @@ From LinearCore Require Import
 
 
 Definition to : Type -> Type := MapCore.t.
-Arguments to T.
+Arguments to T : simpl never.
 
 Definition set := to unit.
 Arguments set/.
@@ -16,10 +16,10 @@ Arguments set/.
 
 
 Definition Find {T} (m : to T) k v := MapCore.MapsTo k v m.
-Arguments Find {T} m k v.
+Arguments Find {T} m k v : simpl never.
 
 Definition find {T} (m : to T) k := MapCore.find k m.
-Arguments find {T} m k.
+Arguments find {T} m k : simpl never.
 
 Lemma find_spec {T} (m : to T) k
   : Reflect.Option (Find m k) (find m k).
@@ -29,7 +29,7 @@ Proof.
   - intros v M. apply MapCore.find_spec in M. rewrite M in F. discriminate F.
 Qed.
 
-Lemma find_det {T} (m : to T) k v1 (F1 : Find m k v1) v2 (F2 : Find m k v2)
+Lemma find_det {T} {m : to T} {k v1} (F1 : Find m k v1) {v2} (F2 : Find m k v2)
   : v1 = v2.
 Proof.
   unfold Find in *. apply MapCore.find_spec in F1. apply MapCore.find_spec in F2.
@@ -63,8 +63,8 @@ Qed.
 Definition ForAll {T} (P : Name.name -> T -> Prop) (m : to T) : Prop :=
   forall k v (F : Find m k v), P k v.
 
-Definition for_all : forall {T}, (Name.name -> T -> bool) -> to T -> bool := @MapCore.for_all.
-Arguments for_all/ {T} p m : rename.
+Definition for_all : forall T, (Name.name -> T -> bool) -> to T -> bool := @MapCore.for_all.
+Arguments for_all {T} p m : rename, simpl never.
 
 Lemma for_all_spec {T P p} (R : forall k (v : T), Reflect.Bool (P k v) (p k v)) m
   : Reflect.Bool (ForAll P m) (for_all p m).
@@ -126,13 +126,21 @@ Lemma eq_spec {T eqb} (eqb_spec : forall a b : T, Reflect.Bool (a = b) (eqb a b)
   : Reflect.Bool (Eq a b) (eq eqb a b).
 Proof. eapply Reflect.bool_eq. { apply eq_both_subset. } apply Reflect.and; apply subset_spec; exact eqb_spec. Qed.
 
+Lemma eq_refl {T} (m : to T)
+  : Eq m m.
+Proof. split; intro F; exact F. Qed.
+
+Lemma eq_sym {T} (a b : to T)
+  : Eq a b <-> Eq b a.
+Proof. split; intros E k v; cbn in E; rewrite E; reflexivity. Qed.
+
 
 
 Definition Empty {T} (m : to T) : Prop :=
   forall k (I : In m k), False.
 
 Definition empty := @MapCore.empty.
-Arguments empty/ {T} : rename.
+Arguments empty {T} : rename, simpl never.
 
 Lemma empty_empty {T} : Empty (@empty T).
 Proof. intros k [v F]. invert F. Qed.
@@ -141,9 +149,10 @@ Proof. intros k [v F]. invert F. Qed.
 
 Definition Singleton {T} k v (m : to T) : Prop :=
   forall x y, Find m x y <-> (x = k /\ y = v).
+Arguments Singleton {T} k v m/.
 
-Definition singleton : forall {T}, Name.name -> T -> to T := @MapCore.singleton.
-Arguments singleton {T} k v.
+Definition singleton : forall T, Name.name -> T -> to T := @MapCore.singleton.
+Arguments singleton {T} k v : simpl never.
 
 Lemma find_singleton {T} x y k (v : T)
   : Find (singleton k v) x y <-> (x = k /\ y = v).
@@ -158,10 +167,20 @@ Lemma in_singleton {T} x k (v : T)
   : In (singleton k v) x <-> x = k.
 Proof.
   split.
-  - intros [y M]. apply MapCore.bindings_spec1 in M. rewrite MapCore.singleton_spec in M.
-    invert M as [? ? E | ? ? C]. 2: { invert C. } invert E as [Ex Ey]. exact Ex.
+  - intros [y F]. apply MapCore.bindings_spec1 in F. rewrite MapCore.singleton_spec in F.
+    invert F as [? ? E | ? ? C]. 2: { invert C. } invert E as [Ex Ey]. exact Ex.
   - intros ->. eexists. apply MapCore.bindings_spec1. left. split; reflexivity.
 Qed.
+
+Lemma singleton_singleton k {T} (v : T)
+  : Singleton k v (singleton k v).
+Proof. cbn. intros. apply find_singleton. Qed.
+
+Lemma singleton_det k {T} (v : T)
+  m1 (S1 : Singleton k v m1)
+  m2 (S2 : Singleton k v m2)
+  : Eq m1 m2.
+Proof. cbn in *. intros. rewrite S1. rewrite S2. reflexivity. Qed.
 
 
 
@@ -193,8 +212,8 @@ Arguments Add {T} k v m m'/.
 (* Cool etymology: <https://www.etymonline.com/word/override>
  * And regarding distinction with "overwrite" (nowhere online has sources, but I think it makes sense):
  * <https://stackoverflow.com/questions/8651562/overwrite-or-override> *)
-Definition overriding_add : forall {T}, Name.name -> T -> to T -> to T := @MapCore.add.
-Arguments overriding_add {T} k v m.
+Definition overriding_add : forall T, Name.name -> T -> to T -> to T := @MapCore.add.
+Arguments overriding_add {T} k v m : simpl never.
 
 Definition checked_add {T} (eqb : T -> T -> bool) k v (m : to T) :=
   match find m k with
@@ -203,15 +222,112 @@ Definition checked_add {T} (eqb : T -> T -> bool) k v (m : to T) :=
   end.
 Arguments checked_add {T} eqb k v m/.
 
-Lemma in_add {T} x k v (m : to T)
+Definition disjoint_add {T} k v (m : to T) :=
+  match find m k with
+  | None => Some (overriding_add k v m)
+  | Some v' => None
+  end.
+Arguments disjoint_add {T} k v m/.
+
+Lemma find_overriding_add {T} {k v} {m : to T} (A : AgreeOn k v m) x y
+  : Find (overriding_add k v m) x y <-> ((x = k /\ y = v) \/ Find m x y).
+Proof.
+  split.
+  - intro M. apply MapCore.find_spec in M. destruct (Name.spec x k); [left | right].
+    + subst. split. { reflexivity. } unfold overriding_add in M.
+      rewrite MapCore.add_spec1 in M. { invert M. subst. reflexivity. }
+    + rewrite MapCore.add_spec2 in M. 2: { symmetry. exact N. } apply MapCore.find_spec. exact M.
+  - intros [[-> ->] | M]. { apply MapCore.find_spec. apply MapCore.add_spec1. }
+    destruct (Name.spec x k). { subst. apply MapCore.find_spec. erewrite (A _ M). apply MapCore.add_spec1. }
+    apply MapCore.find_spec. rewrite MapCore.add_spec2. 2: { symmetry. exact N. } apply MapCore.find_spec. exact M.
+Qed.
+
+Lemma in_overriding_add {T} x k v (m : to T)
   : In (overriding_add k v m) x <-> (x = k \/ In m x).
 Proof.
   split.
-  - intros [y M]. apply MapCore.find_spec in M. destruct (Name.spec x k); [left | right]. { exact Y. }
-    rewrite MapCore.add_spec2 in M. 2: { symmetry. exact N. } eexists. apply MapCore.find_spec. exact M.
-  - intros [-> | [y M]]. { eexists. apply MapCore.find_spec. apply MapCore.add_spec1. }
+  - intros [y F]. apply MapCore.find_spec in F. destruct (Name.spec x k); [left | right]. { exact Y. }
+    rewrite MapCore.add_spec2 in F. 2: { symmetry. exact N. } eexists. apply MapCore.find_spec. exact F.
+  - intros [-> | [y F]]. { eexists. apply MapCore.find_spec. apply MapCore.add_spec1. }
     destruct (Name.spec x k). { subst. eexists. apply MapCore.find_spec. apply MapCore.add_spec1. }
-    eexists. apply MapCore.find_spec. rewrite MapCore.add_spec2. 2: { symmetry. exact N. } apply MapCore.find_spec. exact M.
+    eexists. apply MapCore.find_spec. rewrite MapCore.add_spec2. 2: { symmetry. exact N. }
+    apply MapCore.find_spec. exact F.
+Qed.
+
+Lemma add_overriding {T} {k v} {m : to T} (A : AgreeOn k v m)
+  : Add k v m (overriding_add k v m).
+Proof. cbn. intros. rewrite find_overriding_add. { reflexivity. } exact A. Qed.
+
+Lemma find_checked_add {T eqb} (eqb_spec : forall a b, Reflect.Bool (a = b) (eqb a b))
+  {k v} {m m' : to T} (E : checked_add eqb k v m = Some m') x y
+  : Find m' x y <-> ((x = k /\ y = v) \/ Find m x y).
+Proof.
+  unfold checked_add in E. destruct (find_spec m k) as [v' M | N].
+  - destruct (eqb_spec v' v); invert E. split. { intro F. right. exact F. }
+    intros [[-> ->] | F]. { exact M. } exact F.
+  - invert E. apply find_overriding_add. cbn. intros. apply N in F as [].
+Qed.
+
+Lemma in_checked_add {T eqb} (eqb_spec : forall a b, Reflect.Bool (a = b) (eqb a b))
+  {k v} {m m' : to T} (E : checked_add eqb k v m = Some m') x
+  : In m' x <-> (x = k \/ In m x).
+Proof.
+  unfold checked_add in E. destruct (find_spec m k) as [v' M | N].
+  - destruct (eqb_spec v' v); invert E. split. { intro F. right. exact F. }
+    intros [-> | F]. { eexists. exact M. } exact F.
+  - invert E. apply in_overriding_add.
+Qed.
+
+Lemma add_checked {T eqb} (eqb_spec : forall a b, Reflect.Bool (a = b) (eqb a b))
+  {k v} {m m' : to T} (E : checked_add eqb k v m = Some m')
+  : Add k v m m'.
+Proof.
+  unfold checked_add in E. destruct (find_spec m k) as [v' M | N].
+  - destruct (eqb_spec v' v); invert E. split. { intro F. right. exact F. }
+    intros [[-> ->] | F]. { exact M. } exact F.
+  - invert E. apply add_overriding. cbn. intros. apply N in F as [].
+Qed.
+
+Lemma find_disjoint_add {T k v} {m m' : to T} (E : disjoint_add k v m = Some m') x y
+  : Find m' x y <-> ((x = k /\ y = v) \/ Find m x y).
+Proof.
+  unfold disjoint_add in E. destruct (find_spec m k) as [v' M | N]. { discriminate E. }
+  invert E. apply find_overriding_add. cbn. intros. apply N in F as [].
+Qed.
+
+Lemma in_disjoint_add {T k v} {m m' : to T} (E : disjoint_add k v m = Some m') x
+  : In m' x <-> (x = k \/ In m x).
+Proof.
+  unfold disjoint_add in E. destruct (find_spec m k) as [v' M | N]. { discriminate E. }
+  invert E. apply in_overriding_add.
+Qed.
+
+Lemma add_disjoint {T k v} {m m' : to T} (E : disjoint_add k v m = Some m')
+  : Add k v m m'.
+Proof.
+  unfold disjoint_add in E. destruct (find_spec m k) as [v' M | N].
+  invert E. invert E. apply add_overriding. cbn. intros. apply N in F as [].
+Qed.
+
+Lemma add_det
+  k1 {T} (v1 : T) m1 m1' (A1 : Add k1 v1 m1 m1')
+  k2 (Ek : k1 = k2)
+  v2 (Ev : v1 = v2)
+  m2 (Em : Eq m1 m2)
+  m2' (A2 : Add k2 v2 m2 m2')
+  : Eq m1' m2'.
+Proof. cbn in *. intros x y. subst. rewrite A1. rewrite A2. rewrite Em. reflexivity. Qed.
+
+Lemma add_eq
+  k1 {T} (v1 : T) m1 m' (A1 : Add k1 v1 m1 m')
+  k2 (Ek : k1 = k2)
+  v2 (Ev : v1 = v2)
+  m2 (Em : Eq m1 m2)
+  : Add k2 v2 m2 m'.
+Proof.
+  subst. split.
+  - intro F. apply A1 in F as [[-> ->] | F]; [left | right]. { split; reflexivity. } apply Em. exact F.
+  - intro F. apply A1. destruct F as [[-> ->] | F]; [left | right]. { split; reflexivity. } apply Em. exact F.
 Qed.
 
 
@@ -241,12 +357,12 @@ Lemma union_agree {T} {a b c : to T} (U : Union a b c)
   : Agree a b.
 Proof. cbn. intros. eapply find_det; apply U; [right | left]; eassumption. Qed.
 
-Definition override {T} (_ : Name.name) (a b : option T) :=
+Definition override {T} {_ : Name.name} (a b : option T) :=
   match a with Some y => Some y | None => b end.
-Arguments override {T} _ a/ b.
+Arguments override {T _} a/ b.
 
-Definition overriding_union {T} : to T -> to T -> to T := @MapCore.merge T T T override.
-Arguments overriding_union {T} a b : rename.
+Definition overriding_union {T} : to T -> to T -> to T := @MapCore.merge T T T (@override _).
+Arguments overriding_union {T} a b : rename, simpl never.
 
 Definition set_union : set -> set -> set := overriding_union.
 Arguments set_union/ a b.
@@ -259,19 +375,32 @@ Lemma find_overriding_union {T} (a b : to T) x
 Proof.
   unfold overriding_union. destruct (find_spec a x) as [y M | Na].
   - assert (I : In a x). { eexists. exact M. } unfold find.
-    edestruct (@MapCore.merge_spec1 _ _ _ override a b _ (or_introl I)) as [? [-> ->]].
+    edestruct (@MapCore.merge_spec1 _ _ _ (@override _) a b _ (or_introl I)) as [? [-> ->]].
     cbn. apply find_iff in M. unfold find in M. rewrite M. reflexivity.
   - destruct (find_spec b x) as [y M | Nb].
     + assert (I : In b x). { eexists. exact M. } unfold find.
-      edestruct (@MapCore.merge_spec1 _ _ _ override a b _ (or_intror I)) as [? [-> ->]].
+      edestruct (@MapCore.merge_spec1 _ _ _ (@override _) a b _ (or_intror I)) as [? [-> ->]].
       cbn. destruct MapCore.find eqn:F. { apply MapCore.find_spec in F. apply Na in F as []. }
       apply MapCore.find_spec. exact M.
     + destruct find eqn:F. 2: { reflexivity. }
-      apply MapCore.find_spec in F. assert (I : In (MapCore.merge override a b) x). { eexists. exact F. }
+      apply MapCore.find_spec in F. assert (I : In (MapCore.merge (@override T) a b) x). { eexists. exact F. }
       apply MapCore.merge_spec2 in I as [[y M] | [y M]]; [apply Na in M as [] | apply Nb in M as []].
 Qed.
 
-Lemma union_overriding_union {T} (a b : to T) (A : Agree a b)
+Lemma in_overriding_union {T} (a b : to T) x
+  : In (overriding_union a b) x <-> In a x \/ In b x.
+Proof.
+  split.
+  - intros [y F]. apply find_iff in F. rewrite find_overriding_union in F.
+    destruct (find_spec a x). { invert F. left. eexists. exact Y. } right. eexists. apply find_iff. exact F.
+  - intros [[y F] | [y F]].
+    + eexists; apply find_iff; rewrite find_overriding_union. apply find_iff in F. rewrite F. reflexivity.
+    + destruct (find_spec a x); eexists; apply find_iff; rewrite find_overriding_union.
+      * apply find_iff in Y. rewrite Y. reflexivity.
+      * destruct (find_spec a x). { apply N in Y as []. } apply find_iff. exact F.
+Qed.
+
+Lemma union_overriding_union {T} {a b : to T} (A : Agree a b)
   : Union a b (overriding_union a b).
 Proof.
   split.
@@ -292,7 +421,7 @@ Lemma union_checked_union {T eqb} (eqb_spec : forall a b : T, Reflect.Bool (a = 
   : Union a b c.
 Proof. unfold checked_union in E. destruct (agree_spec eqb_spec a b); invert E. apply union_overriding_union. exact Y. Qed.
 
-Lemma union_iff {T eqb} (eqb_spec : forall a b : T, Reflect.Bool (a = b) (eqb a b)) {a b c : to T}
+Lemma union_iff {T eqb} (eqb_spec : forall a b : T, Reflect.Bool (a = b) (eqb a b)) (a b c : to T)
   : Union a b c <-> exists c', (checked_union eqb a b = Some c' /\ Eq c c').
 Proof.
   unfold Union. unfold checked_union. unfold Eq. destruct (agree_spec eqb_spec a b). 2: {
@@ -301,3 +430,9 @@ Proof.
     split. { intros [? [tmp E]]; invert tmp. exact E. } intro E. eexists. split. { reflexivity. } exact E. }
   split; intros U' k v; rewrite U'; [symmetry |]; apply union_overriding_union; exact Y.
 Qed.
+
+
+
+Definition Reflect (P : Name.name -> Prop) (p : set) : Prop :=
+  forall x, (In p x <-> P x).
+Arguments Reflect P p/.
