theories/Match.v
@@ -9,24 +9,87 @@ From LinearCore Require Import
 
 
 
-Inductive Raw : forall (pattern : Pattern.raw) (term : Term.term) (matches : Map.to Term.term), Prop :=
+Inductive Strict : Pattern.strict -> Term.term -> Map.to Term.term -> Prop :=
   | Ctr matches (E : Map.Empty matches) ctor
-      : Raw (Pattern.Ctr ctor) (Term.Ctr ctor) matches
+      : Strict (Pattern.Ctr ctor) (Term.Ctr ctor) matches
   | App
-      function_pattern function function_matches (function_matched : Raw function_pattern function function_matches)
+      function_pattern function function_matches (function_matched : Strict function_pattern function function_matches)
       argument_name (N : forall (I : Map.In function_matches argument_name), False)
       (* can't match the same name twice in the same pattern ^^^ *)
       argument matches (A : Map.Add argument_name argument function_matches matches)
-      : Raw (Pattern.App function_pattern argument_name) (Term.App function argument) matches
+      : Strict (Pattern.App function_pattern argument_name) (Term.App function argument) matches
   .
+Arguments Strict strict term matches.
 
-Fixpoint raw pattern term :=
+Fixpoint strict pattern term : option (Map.to Term.term) :=
   match pattern, term with
   | Pattern.Ctr constructor_pattern, Term.Ctr constructor =>
       if Constructor.eq constructor_pattern constructor then Some Map.empty else None
   | Pattern.App function_pattern argument_name, Term.App function argument =>
-      match raw function_pattern function with None => None | Some function_matches =>
-        Map.checked_add Term.eq argument_name argument function_matches
+      match strict function_pattern function with None => None | Some function_matches =>
+        Map.disjoint_add argument_name argument function_matches
       end
   | _, _ => None
   end.
+
+Lemma strict_det pattern term
+  matches1 (S1 : Strict pattern term matches1)
+  matches2 (S2 : Strict pattern term matches2)
+  : Map.Eq matches1 matches2.
+Proof.
+  generalize dependent matches2. induction S1; intros; invert S2.
+  - split; intro F; [contradiction (E k) | contradiction (E0 k)]; eexists; eassumption.
+  - eapply Map.add_det; [exact A | reflexivity | reflexivity | apply Map.eq_refl |].
+    eapply Map.add_eq; [exact A0 | reflexivity | reflexivity |].
+    apply Map.eq_sym. apply IHS1. exact function_matched.
+Qed.
+
+Lemma strict_spec pattern term
+  : Reflect.Option (Strict pattern term) (strict pattern term).
+Proof.
+  generalize dependent term. induction pattern; intros;
+  destruct term; try solve [constructor; intros t C; invert C].
+  - unfold strict. destruct (Constructor.eq_spec constructor constructor0); constructor.
+    + subst. constructor. apply Map.empty_empty.
+    + intros t C. invert C. apply N. reflexivity.
+
+  - (* See if the curried constructor matched successfully: *)
+    simpl strict. destruct (IHpattern term1) as [function_matches function_matched | N]. 2: {
+      constructor. intros t C. invert C. apply N in function_matched as []. }
+
+    (* See if `argument` was already in `function_matches` (i.e. duplicated, i.e. bad) *)
+    destruct (Map.find_spec function_matches argument) as [duplicated F | N]. 2: {
+      constructor. econstructor. { eassumption. } { intros [y F]. apply N in F as []. }
+      apply Map.add_overriding. cbn. intros. apply N in F as []. }
+    constructor. intros t C. invert C. apply N; clear N. eexists. eapply strict_det; [| | eassumption]; eassumption.
+Qed.
+
+
+
+Variant Pattern : Pattern.pattern -> Term.term -> Map.to Term.term -> Prop :=
+  | Nam name term matches (S : Map.Singleton name term matches)
+      : Pattern (Pattern.Nam name) term matches
+  | Pat strict term matches (strict_matched : Strict strict term matches)
+      : Pattern (Pattern.Pat strict) term matches
+  .
+Arguments Pattern pattern term matches.
+
+Definition pattern patt term :=
+  match patt with
+  | Pattern.Nam name => Some (Map.singleton name term)
+  | Pattern.Pat s => strict s term
+  end.
+
+Lemma pattern_det patt term
+  matches1 (S1 : Pattern patt term matches1)
+  matches2 (S2 : Pattern patt term matches2)
+  : Map.Eq matches1 matches2.
+Proof. invert S1; invert S2. { eapply Map.singleton_det; eassumption. } eapply strict_det; eassumption. Qed.
+
+Lemma pattern_spec patt term
+  : Reflect.Option (Pattern patt term) (pattern patt term).
+Proof.
+  destruct patt; cbn. { constructor. constructor. apply Map.singleton_singleton. }
+  destruct (strict_spec strict0 term); constructor. { constructor. exact Y. }
+  intros m C. invert C. apply N in strict_matched as [].
+Qed.
