theories/Pattern.v
@@ -2,37 +2,61 @@ From LinearCore Require
   Constructor
   Name
   .
+From LinearCore Require Import
+  Invert
+  .
 
 
 
-Inductive raw : Set :=
+Inductive strict : Set :=
   | Ctr (constructor : Constructor.constructor)
-  | App (curried : raw) (argument : Name.name)
+  | App (curried : strict) (argument : Name.name)
   .
 
-Inductive BoundIn : raw -> Name.name -> Prop :=
-  | SArg curried name
-      : BoundIn (App curried name) name
-  | SRec curried name (bound_earlier : BoundIn curried name) argument
-      : BoundIn (App curried argument) name
-  .
-Arguments BoundIn raw name.
-
-Inductive WellFormed : raw -> Prop :=
-  | WFCtr constructor
-      : WellFormed (Ctr constructor)
-  | WFApp curried argument (no_dup_name : forall (B : BoundIn curried argument), False)
-      : WellFormed (App curried argument)
-  .
-Arguments WellFormed raw.
 
 
+Fixpoint strict_eq a b :=
+  match a, b with
+  | Ctr a, Ctr b => Constructor.eq a b
+  | App ca aa, App cb ab => andb (strict_eq ca cb) (Name.eqb aa ab)
+  | _, _ => false
+  end.
+Arguments strict_eq a b.
 
-Definition strict : Type := { raw : raw | WellFormed raw }.
+Lemma strict_eq_spec a b
+  : Reflect.Bool (a = b) (strict_eq a b).
+Proof.
+  generalize dependent b. induction a; intros; destruct b.
+  - unfold strict_eq. destruct (Constructor.eq_spec constructor constructor0); constructor. { subst. reflexivity. }
+    intro E. apply N. invert E. reflexivity.
+  - constructor. intro D. discriminate D.
+  - constructor. intro D. discriminate D.
+  - simpl strict_eq. destruct (IHa b). 2: { constructor. intro E. apply N. invert E. reflexivity. }
+    destruct (Name.spec argument argument0); constructor. { subst. reflexivity. } intro E. apply N. invert E. reflexivity.
+Qed.
 
 
 
-Variant pattern : Type :=
+Variant pattern : Set :=
   | Nam (name : Name.name)
   | Pat (strict : strict)
   .
+
+
+
+Definition eq a b :=
+  match a, b with
+  | Nam a, Nam b => Name.eqb a b
+  | Pat a, Pat b => strict_eq a b
+  | _, _ => false
+  end.
+
+Lemma eq_spec a b
+  : Reflect.Bool (a = b) (eq a b).
+Proof.
+  destruct a; destruct b; cbn.
+  - destruct (Name.spec name name0); constructor. { subst. reflexivity. } intro E. apply N. invert E. reflexivity.
+  - constructor. intro D. discriminate D.
+  - constructor. intro D. discriminate D.
+  - destruct (strict_eq_spec strict0 strict1); constructor. { subst. reflexivity. } intro E. apply N. invert E. reflexivity.
+Qed.
