theories/Term.v
@@ -9,7 +9,7 @@ From LinearCore Require Import
 
 
 
-Inductive term : Type :=
+Inductive term : Set :=
   | Err
   | Typ
   | Prp
@@ -31,7 +31,7 @@ Fixpoint eq a b :=
   | Ref a, Ref b => Name.eqb a b
   | App fa aa, App fb ab => andb (eq fa fb) (eq aa ab)
   | For va ta ba, For vb tb bb => andb (Name.eqb va vb) (andb (eq ta tb) (eq ba bb))
-  | Cas pa ba oa, For pb bb ob => andb (Pattern.eq pa pb) (andb (eq ba bb) (eq oa ob))
+  | Cas pa ba oa, Cas pb bb ob => andb (Pattern.eq pa pb) (andb (eq ba bb) (eq oa ob))
   | _, _ => false
   end.
 
@@ -51,7 +51,7 @@ Proof.
   - simpl eq. destruct (Name.spec variable variable0); cbn in *. 2: { constructor. intro E. apply N. invert E. reflexivity. }
     destruct (IHa1 b1); cbn. 2: { constructor. intro E. apply N. invert E. reflexivity. }
     subst. destruct (IHa2 b2); constructor. { f_equal. assumption. } intro E. apply N. invert E. reflexivity.
-  - simpl eq. destruct (Name.spec variable variable0); cbn in *. 2: { constructor. intro E. apply N. invert E. reflexivity. }
+  - simpl eq. destruct (Pattern.eq_spec pattern pattern0); cbn in *. 2: { constructor. intro E. apply N. invert E. reflexivity. }
     destruct (IHa1 b1); cbn. 2: { constructor. intro E. apply N. invert E. reflexivity. }
     subst. destruct (IHa2 b2); constructor. { f_equal. assumption. } intro E. apply N. invert E. reflexivity.
 Qed.
